code/mpfr/MPFR.Dyadic.fst
@@ -78,6 +78,17 @@ let fmul a b =
     lemma_pow2_mul (a.exponent - elb) (b.exponent - elb);
     mk_dyadic (a.significand * b.significand) (a.exponent + b.exponent)
 
+(* Pow2 Division post-condition
+ * a.mant * 2 ^ (a.exp - elb) = r.mant * 2 ^ (r.exp - elb) * 2 ^ e
+ * is equivalent to
+ * a.mant * 2 ^ a.exp / 2 ^ e = r.mant * 2 ^ r.exp *)
+val fdiv_pow2: a:dyadic -> e:nat -> Tot (r:dyadic{
+    let elb = a.exponent - e in
+    r.exponent >= elb /\
+    eval_i a elb = eval_i r elb * pow2 e})
+    
+let fdiv_pow2 a e = mk_dyadic a.significand (a.exponent - e)
+
 (* Infix notations *)
 unfold let op_Equals_Dot  = eq
 unfold let op_Greater_Dot  = gt
@@ -95,6 +106,26 @@ val dyadic_eq_symm_lemma: a:dyadic -> b:dyadic -> Lemma
     (ensures  (b =. a))
     [SMTPat (a =. b)]
 let dyadic_eq_symm_lemma a b = ()
+
+val dyadic_gt_symm_lemma: a:dyadic -> b:dyadic -> Lemma
+    (requires (a >. b))
+    (ensures  (b <. a))
+let dyadic_gt_symm_lemma a b = ()
+
+val dyadic_ge_symm_lemma: a:dyadic -> b:dyadic -> Lemma
+    (requires (a >=. b))
+    (ensures  (b <=. a))
+let dyadic_ge_symm_lemma a b = ()
+
+val dyadic_lt_symm_lemma: a:dyadic -> b:dyadic -> Lemma
+    (requires (a <. b))
+    (ensures  (b >. a))
+let dyadic_lt_symm_lemma a b = ()
+
+val dyadic_le_symm_lemma: a:dyadic -> b:dyadic -> Lemma
+    (requires (a <=. b))
+    (ensures  (b >=. a))
+let dyadic_le_symm_lemma a b = ()
 
 val dyadic_eq_trans_lemma: a:dyadic -> b:dyadic -> c:dyadic -> Lemma
     (requires (a =. b /\ b =. c))
@@ -212,82 +243,6 @@ let fadd_eq_lemma a b c =
     lemma_pow2_mul (b.exponent - elbbc) (elbbc - elb);
     lemma_pow2_mul (c.exponent - elbbc) (elbbc - elb)
 
-val fadd_gt_lemma: a:dyadic -> b:dyadic -> c:dyadic -> Lemma
-    (requires (b >. c))
-    (ensures  (a +. b >. a +. c))
-    [SMTPat (a +. b); SMTPat (b >. c); SMTPat (a +. c)]
-
-let fadd_gt_lemma a b c =
-    let elbab = min a.exponent b.exponent in
-    let elbac = min a.exponent c.exponent in
-    let elbbc = min b.exponent c.exponent in
-    let elb = min elbab elbac in
-    lemma_distr_add_right (pow2 (elbab - elb)) (a.significand * pow2 (a.exponent - elbab)) (b.significand * pow2 (b.exponent - elbab));
-    lemma_pow2_mul (a.exponent - elbab) (elbab - elb);
-    lemma_pow2_mul (b.exponent - elbab) (elbab - elb);
-    lemma_distr_add_right (pow2 (elbac - elb)) (a.significand * pow2 (a.exponent - elbac)) (c.significand * pow2 (c.exponent - elbac));
-    lemma_pow2_mul (a.exponent - elbac) (elbac - elb);
-    lemma_pow2_mul (c.exponent - elbac) (elbac - elb);
-    lemma_pow2_mul (b.exponent - elbbc) (elbbc - elb);
-    lemma_pow2_mul (c.exponent - elbbc) (elbbc - elb)
-
-val fadd_ge_lemma: a:dyadic -> b:dyadic -> c:dyadic -> Lemma
-    (requires (b >=. c))
-    (ensures  (a +. b >=. a +. c))
-    [SMTPat (a +. b); SMTPat (b >=. c); SMTPat (a +. c)]
-
-let fadd_ge_lemma a b c =
-    let elbab = min a.exponent b.exponent in
-    let elbac = min a.exponent c.exponent in
-    let elbbc = min b.exponent c.exponent in
-    let elb = min elbab elbac in
-    lemma_distr_add_right (pow2 (elbab - elb)) (a.significand * pow2 (a.exponent - elbab)) (b.significand * pow2 (b.exponent - elbab));
-    lemma_pow2_mul (a.exponent - elbab) (elbab - elb);
-    lemma_pow2_mul (b.exponent - elbab) (elbab - elb);
-    lemma_distr_add_right (pow2 (elbac - elb)) (a.significand * pow2 (a.exponent - elbac)) (c.significand * pow2 (c.exponent - elbac));
-    lemma_pow2_mul (a.exponent - elbac) (elbac - elb);
-    lemma_pow2_mul (c.exponent - elbac) (elbac - elb);
-    lemma_pow2_mul (b.exponent - elbbc) (elbbc - elb);
-    lemma_pow2_mul (c.exponent - elbbc) (elbbc - elb)
-
-val fadd_lt_lemma: a:dyadic -> b:dyadic -> c:dyadic -> Lemma
-    (requires (b <. c))
-    (ensures  (a +. b <. a +. c))
-    [SMTPat (a +. b); SMTPat (b <. c); SMTPat (a +. c)]
-
-let fadd_lt_lemma a b c =
-    let elbab = min a.exponent b.exponent in
-    let elbac = min a.exponent c.exponent in
-    let elbbc = min b.exponent c.exponent in
-    let elb = min elbab elbac in
-    lemma_distr_add_right (pow2 (elbab - elb)) (a.significand * pow2 (a.exponent - elbab)) (b.significand * pow2 (b.exponent - elbab));
-    lemma_pow2_mul (a.exponent - elbab) (elbab - elb);
-    lemma_pow2_mul (b.exponent - elbab) (elbab - elb);
-    lemma_distr_add_right (pow2 (elbac - elb)) (a.significand * pow2 (a.exponent - elbac)) (c.significand * pow2 (c.exponent - elbac));
-    lemma_pow2_mul (a.exponent - elbac) (elbac - elb);
-    lemma_pow2_mul (c.exponent - elbac) (elbac - elb);
-    lemma_pow2_mul (b.exponent - elbbc) (elbbc - elb);
-    lemma_pow2_mul (c.exponent - elbbc) (elbbc - elb)
-
-val fadd_le_lemma: a:dyadic -> b:dyadic -> c:dyadic -> Lemma
-    (requires (b <=. c))
-    (ensures  (a +. b <=. a +. c))
-    [SMTPat (a +. b); SMTPat (b <=. c); SMTPat (a +. c)]
-
-let fadd_le_lemma a b c =
-    let elbab = min a.exponent b.exponent in
-    let elbac = min a.exponent c.exponent in
-    let elbbc = min b.exponent c.exponent in
-    let elb = min elbab elbac in
-    lemma_distr_add_right (pow2 (elbab - elb)) (a.significand * pow2 (a.exponent - elbab)) (b.significand * pow2 (b.exponent - elbab));
-    lemma_pow2_mul (a.exponent - elbab) (elbab - elb);
-    lemma_pow2_mul (b.exponent - elbab) (elbab - elb);
-    lemma_distr_add_right (pow2 (elbac - elb)) (a.significand * pow2 (a.exponent - elbac)) (c.significand * pow2 (c.exponent - elbac));
-    lemma_pow2_mul (a.exponent - elbac) (elbac - elb);
-    lemma_pow2_mul (c.exponent - elbac) (elbac - elb);
-    lemma_pow2_mul (b.exponent - elbbc) (elbbc - elb);
-    lemma_pow2_mul (c.exponent - elbbc) (elbbc - elb)
-
 val fadd_comm_lemma: a:dyadic -> b:dyadic -> Lemma
     (a +. b =. b +. a)
     [SMTPat (a +. b)]
@@ -308,9 +263,3 @@ let fadd_asso_lemma a b c =
     lemma_distr_add_right (pow2 (elbbc - elb)) (b.significand * pow2 (b.exponent - elbbc)) (c.significand * pow2 (c.exponent - elbbc));
     lemma_pow2_mul (b.exponent - elbbc) (elbbc - elb);
     lemma_pow2_mul (c.exponent - elbbc) (elbbc - elb)
-
-val fadd_zero_lemma: a:dyadic -> Lemma
-    (a +. zero_dyadic =. a)
-    [SMTPat (a +. zero_dyadic)]
-
-let fadd_zero_lemma a = ()
