code/mpfr/MPFR.Exceptions.fst
@@ -23,25 +23,52 @@ open MPFR.Exceptions.Lemma
 
 val mpfr_overflow: x:mpfr_ptr -> rnd_mode:mpfr_rnd_t -> sign:mpfr_sign_t ->
     Stack i32
-    (requires (fun h -> let p = (as_struct h x).mpfr_prec in
-                     let l = (U32.v p - 1) / 64 + 1 in
-                     mpfr_live h x /\ mpfr_PREC_COND (U32.v p) /\
-		     length (as_struct h x).mpfr_d = l))
-    (ensures  (fun h0 f h1 ->
+    (requires (fun h -> 
+        let p = (as_struct h x).mpfr_prec in
+        let l = (U32.v p - 1) / 64 + 1 in
+        mpfr_live h x /\ mpfr_PREC_COND (U32.v p) /\
+	length (as_struct h x).mpfr_d = l))
+    (ensures  (fun h0 t h1 ->
         let p = (as_struct h1 x).mpfr_prec in
         mpfr_live h1 x /\ mpfr_modifies x h0 h1 /\
         mpfr_valid_cond h1 x /\ (as_struct h1 x).mpfr_sign = sign /\
 	(forall (exact:normal_fp{exact.sign = I32.v sign /\ exact.exp > mpfr_EMAX_spec /\
 	                    exact.prec >= U32.v p}).
 	as_fp h1 x == mpfr_overflow_spec exact (U32.v p) rnd_mode /\
-	I32.v f = mpfr_overflow_ternary_spec exact (U32.v p) rnd_mode)))
+	I32.v t = mpfr_overflow_ternary_spec exact (U32.v p) rnd_mode)))
 
 let mpfr_overflow x rnd_mode sign =
     mpfr_SET_SIGN x sign;
-    if mpfr_IS_LIKE_RNDZ rnd_mode (sign = mpfr_SIGN_NEG) then begin
+    if mpfr_IS_LIKE_RNDZ rnd_mode (mpfr_IS_NEG_SIGN sign) then begin
 	mpfr_setmax x;
 	mpfr_NEG_SIGN sign
     end else begin
         mpfr_SET_INF x;
+	sign
+    end
+
+val mpfr_underflow: x:mpfr_ptr -> rnd_mode:mpfr_rnd_t -> sign:mpfr_sign_t ->
+    Stack i32
+    (requires (fun h -> 
+        let p = (as_struct h x).mpfr_prec in
+        let l = (U32.v p - 1) / 64 + 1 in
+        mpfr_live h x /\ mpfr_PREC_COND (U32.v p) /\
+	length (as_struct h x).mpfr_d = l))
+    (ensures  (fun h0 t h1 ->
+        let p = (as_struct h1 x).mpfr_prec in
+        mpfr_live h1 x /\ mpfr_modifies x h0 h1 /\
+        mpfr_valid_cond h1 x /\ (as_struct h1 x).mpfr_sign = sign /\
+	(forall (exact:normal_fp{exact.sign = I32.v sign /\ exact.exp < mpfr_EMIN_spec /\
+	                    exact.prec >= U32.v p}).
+	as_fp h1 x == mpfr_underflow_spec exact (U32.v p) rnd_mode /\
+	I32.v t = mpfr_underflow_ternary_spec exact (U32.v p) rnd_mode)))
+
+let mpfr_underflow x rnd_mode sign =
+    mpfr_SET_SIGN x sign;
+    if mpfr_IS_LIKE_RNDZ rnd_mode (mpfr_IS_NEG_SIGN sign) then begin
+        mpfr_SET_ZERO x;
+	mpfr_NEG_SIGN sign
+    end else begin
+        mpfr_setmin x;
 	sign
     end
